experiment/Experiment.Steel.GCombinators.fst
@@ -1,0 +1,151 @@
+module Experiment.Steel.GCombinators
+
+module U    = Learn.Util
+module L    = FStar.List.Pure
+module M    = Experiment.Steel.Repr.M
+module MC   = Experiment.Steel.Combinators
+module LV   = Experiment.Steel.Repr.LV
+module SF   = Experiment.Steel.Repr.SF
+module SH   = Experiment.Steel.Steel
+module Ll   = Learn.List
+module Fl   = Learn.FList
+module Veq  = Experiment.Steel.VEquiv
+module Mem  = Steel.Memory
+module Perm = Learn.Permutation
+
+open Steel.Effect
+open Steel.Effect.Atomic
+open Experiment.Steel.VPropList
+open Experiment.Steel.Interface
+open FStar.Tactics
+open Experiment.Steel.Tac
+
+#set-options "--fuel 1 --ifuel 1"
+
+#push-options "--fuel 0 --ifuel 0"
+//TODO? inline s
+inline_for_extraction
+let make_combinator_steel_ghost
+      (#a : Type u#a) (opened : Mem.inames) (s : M.spec_r a) (f : M.spc_steel_t (SH.KGhost opened) s)
+      (#pre : M.pre_t) (pre_eq : Veq.vequiv pre (M.spc_pre1 s))
+      (#post : M.post_t a) (post_eq : ((x : a) -> Veq.vequiv (M.spc_post1 s x) (post x)))
+  : M.repr_steel_t (SH.KGhost opened) a pre post (M.gen_req s pre_eq post_eq) (M.gen_ens s pre_eq post_eq)
+  =
+    SH.ghost_f #opened (fun () ->
+      pre_eq.veq_g _;
+      (**) steel_elim_vprop_of_list_append_f s.spc_pre s.spc_ro;
+      (**) let sl0'  = gget_f s.spc_pre in
+      (**) let sl_ro = gget_f s.spc_ro in     
+      (**) assert (s.spc_req sl0' sl_ro);
+      let (x : a) = SH.ghost_u f () in
+      (**) let sl1'   = gget_f (s.spc_post x) in
+      (**) let sl_ro' = gget_f s.spc_ro       in
+      (**) assert (sl_ro' == sl_ro);
+      (**) assert (s.spc_ens sl0' x sl1' sl_ro);
+      (**) steel_intro_vprop_of_list_append_f (s.spc_post x) s.spc_ro;
+      (post_eq x).veq_g _;
+      x
+    )
+#pop-options
+    
+
+(**** slrewrite *)
+
+/// [slrewrite x0 x1] will replace any occurrence of [x0] by [x1] in the current environment (using [l_to_r]).
+/// Requires [x0 == x1].
+
+[@@ Learn.Tactics.Util.__tac_helper__]
+let slrewrite_spec_r (#t : Type u#t) (x0 x1 : t) (v0 v1 frame : vprop_list) (veq : squash (x0 == x1 ==> v0 == v1))
+  : M.spec_r (U.unit' u#a)
+  = M.Mkspec_r
+       v0 (fun _ -> v1) frame
+       (fun _ _ -> x0 == x1)
+       (fun sl0 _ sl1 _ -> x0 == x1 /\ sl1 == sl0)
+
+noeq
+type slrewrite_gen_c (#t : Type u#t) (x0 x1 : t)
+  : M.spec_r (U.unit' u#a) -> Type u#(max a 2) =
+  | SlRewrite : (v0 : vprop_list) -> (v1 : vprop_list) -> (frame : vprop_list) ->
+                (veq : squash (x0 == x1 ==> v0 == v1)) ->
+                slrewrite_gen_c x0 x1 (slrewrite_spec_r x0 x1 v0 v1 frame veq)
+
+let slrewrite_steel
+      (opened : Mem.inames)
+      (#t : Type u#t) (x0 x1 : t) (v0 v1 frame : vprop_list) (veq : squash (x0 == x1 ==> v0 == v1))
+  : M.spc_steel_t (SH.KGhost opened) (slrewrite_spec_r u#t u#a x0 x1 v0 v1 frame veq)
+  = SH.ghost_f #opened (fun () ->
+    change_equal_slprop (vprop_of_list v0) (vprop_of_list v1);
+    U.Unit'
+  )
+
+// TODO: put the unchanged vprop' in the frame
+#push-options "--ifuel 0 --fuel 1"
+[@@__cond_solver__]
+let __build_slrewrite
+      (env : vprop_list)
+      (#t : Type u#t) (x0 x1 : t) (#gen_tac : M.gen_tac_t)
+      (env' : vprop_list)
+      (rew : (rew_x : unit -> Lemma (x0 == x1)) -> squash (env == env'))
+  : LV.lin_cond env (M.Tgen (U.unit' u#a) gen_tac (slrewrite_gen_c #t x0 x1)) (LV.csm_all env) (fun _ -> env')
+  =
+    introduce x0 == x1 ==> env == env'
+      with _ . rew (fun () -> ());
+    let s = slrewrite_spec_r x0 x1 env env' [] () in
+    let sf : LV.gen_sf s =
+      fun sl0 sl_ro ->
+        introduce forall sl1 . Fl.flist_eq2 sl1 sl0 <==> sl1 == sl0
+          with Fl.flist_eq2_spec sl1 sl0;
+        SF.Tspec U.unit' (M.post_sl_t s.spc_post)
+             (x0 == x1) (fun _ sl1 -> x0 == x1 /\ Fl.flist_eq2 sl1 sl0)
+    in
+    let pre_f : Perm.pequiv_list env (M.spc_pre1 s) = Perm.perm_f_to_list (Perm.pequiv_refl env) in
+    Ll.list_extensionality (LV.gen_csm pre_f) (LV.csm_all env) (fun i ->
+      let pre_f' = (LV.eij_split s.spc_pre s.spc_ro (LV.eij_of_perm_l pre_f))._1 in
+      U.assert_by (L.index pre_f' i == i) (fun () ->
+        Ll.splitAt_index (L.length env) (LV.eij_of_perm_l pre_f));
+      L.lemma_index_memP pre_f' i
+    );
+    LV.LCgen env s (SlRewrite env env' [] ()) pre_f sf
+#pop-options
+
+let build_slrewrite (fr : flags_record) : Tac unit
+  =
+    apply (`__build_slrewrite);
+    // rew
+    let rew_x = intro () in
+    l_to_r [binder_to_term rew_x];
+    trefl ()
+
+[@@ M.__repr_M__]
+let slrewrite_M_tree (#t : Type u#t) (x0 x1 : t)
+  : M.prog_tree (U.unit' u#a)
+  = M.Tgen (U.unit' u#a) build_slrewrite (slrewrite_gen_c #t x0 x1)
+
+[@@ M.__repr_M__]
+inline_for_extraction
+let slrewrite (#t : Type u#t) (#opened : Mem.inames) (x0 x1 : t)
+  : M.repr (SH.KGhost opened) (U.unit' u#a)
+  = {
+    repr_tree  = slrewrite_M_tree x0 x1;
+    repr_steel = (fun pre post c ->
+                    let M.TCgen s sh _ pre_eq _ post_eq = c in
+                    let SlRewrite v0 v1 frame veq = U.cast (slrewrite_gen_c #t x0 x1 s) sh in
+                    make_combinator_steel_ghost opened s
+                      (slrewrite_steel opened x0 x1 v0 v1 frame veq)
+                      pre_eq post_eq)
+  }
+
+
+module F   = Experiment.Steel.Notations
+module U32 = FStar.UInt32
+open Steel.Reference
+
+let test_slrewrite (r0 r1 r2 : ref U32.t)
+  : F.steel unit
+      (vptr r0 `star` vptr r1) (fun _ -> vptr r2 `star` vptr r1)
+      (requires fun _ -> r0 == r2)
+      (ensures  fun h0 _ h1 -> sel r0 h0 == sel r2 h1 /\ sel r1 h0 == sel r1 h1)
+  = F.(to_steel (
+      MC.ghost_to_steel_ct (slrewrite r0 r2) (fun _ -> U.Unit');;
+      return ()
+    ) ())
